Fleshing out the BR93 example.

cost.ec
@@ -1,29 +1,101 @@
-require import Int List CHoareTactic StdBigop.
+require import Distr DBool Int List CHoareTactic StdBigop.
 import Bigint IntExtra.
-
-schema plus_cost ['a] {e e' : int}: 
-cost[true : e + e'] = 
-cost[true : e] + cost[true : e'] + 1 .
-print plus_cost.
-
-lemma foo : cost(_:{})[true : 1 + 2] = 1.
-proof.
-instantiate := (plus_cost {} 1 : 2) => H; rewrite H.
-have := a.
-admit.
-qed.
-
-lemma bar : 
-cost(_ : {z : int})[z = 1 : z + 2] = 1.
-proof.
-
-
+require BitWord ROM.
 
 (*****************)
 (* Example BR93: *)
 (*****************)
+
+(* Plaintexts                                                           *)
+op k : { int | 0 < k } as gt0_k.
+
+clone import BitWord as Plaintext with
+  op n <- k
+proof gt0_n by exact/gt0_k
+rename
+  "word" as "ptxt"
+  "dunifin" as "dptxt".
+import DWord.
+
+(* Nonces                                                               *)
+op l : { int | 0 < l } as gt0_l.
+
+clone import BitWord as Randomness with
+  op n <- l
+proof gt0_n by exact/gt0_l
+rename
+  "word" as "rand"
+  "dunifin" as "drand".
+import DWord.
+
+(* Ciphertexts                                                          *)
+op n = l + k.
+lemma gt0_n: 0 < n by smt(gt0_k gt0_l).
+
+clone import BitWord as Ciphertext with
+  op n <- n
+proof gt0_n by exact/Self.gt0_n
+rename "word" as "ctxt".
+
+(* Parsing and Formatting                                               *)
+op (||) (r:rand) (p:ptxt) : ctxt = mkctxt ((ofrand r) ++ (ofptxt p)).
+
+op parse (c:ctxt): rand * ptxt =
+  (mkrand (take l (ofctxt c)),mkptxt (drop l (ofctxt c))).
+
+lemma parseK r p: parse (r || p) = (r,p).
+proof.
+rewrite /parse /(||) ofctxtK 1:size_cat 1:size_rand 1:size_ptxt //=.
+by rewrite take_cat drop_cat size_rand take0 drop0 cats0 mkrandK mkptxtK.
+qed.
+
+lemma formatI (r : rand) (p : ptxt) r' p':
+  (r || p) = (r' || p') => (r,p) = (r',p').
+proof. by move=> h; rewrite -(@parseK r p) -(@parseK r' p') h. qed.
+
+(* A set `pkey * skey` of keypairs, equipped with                       *)
+(*                         a lossless, full, uniform distribution dkeys *)
+type pkey, skey.
+op dkeys: { (pkey * skey) distr |    is_lossless dkeys
+                                  /\ is_funiform dkeys } as dkeys_llfuni.
+
+(* A family `f` of trapdoor permutations over `rand`,                   *)
+(*        indexed by `pkey`, with inverse family `fi` indexed by `skey` *)
+op f : pkey -> rand -> rand.
+op fi: skey -> rand -> rand.
+axiom fK pk sk x: (pk,sk) \in dkeys => fi sk (f pk x) = x.
+
+
+(* Random Oracle                                                        *)
+clone import ROM.Lazy as H with
+  type from      <- rand,
+  type to        <- ptxt,
+  op   dsample _ <- dptxt.
+
+(************************************************************************)
+(* Costs of various operators. *)
+schema cost_cons ['a] {e : 'a} {l : 'a list} : 
+    cost[true : e :: l] =   
+    cost[true : e] + cost[true : l] + 1.
+
+
+schema cost_nil ['a] : cost[true : [] : 'a list] = 1.
+
+schema cost_pp {r : rand} {p : ptxt} :
+  cost[true : r || p] = 
+  cost[true : r] + cost[true : p] + 1.
+
+schema cost_dptxt : cost[true : dptxt] = 1.
+
+
+(************************************************************************)
 module type Oracle = {
-  proc o (x : int) : int
+  proc init () : unit
+  proc o (x : rand) : ptxt
+}.
+
+module type AOracle = {
+  proc o (x : rand) : ptxt
 }.
 
 op k1 : int.
@@ -32,39 +104,38 @@ op k2 : int.
 axiom k1p : 0 <= k1.
 axiom k2p : 0 <= k2.
 
-module type Adv (H : Oracle) = {
-  proc a1(x : int) : int * int
-  proc a2(x : int) : int
+module type Adv (H : AOracle) = {
+  proc a1(p:pkey): (ptxt * ptxt)
+  proc a2(c:ctxt): bool         
 }.
 
-(*****************)
-(* Other example *)
+(*********************************************)
+(* Other example, to the the accepted syntax *)
 
 (* We have two possibility to give module restrictions. *)
 (* We can give the restrictions function by function, e.g.: *)
-module type OAdv (H1 : Oracle) (H : Oracle) = {
-  proc a1(x : int) : int * int {H.o : k1, H1.o : 1} 
-  proc a2(x : int) : int       {H.o : k2, H1.o : 3} 
+module type OAdv (H1 : Oracle) (H : AOracle) = {
+  proc a1(x : pkey) : ptxt * ptxt {H.o : k1, H1.o : 1} 
+  proc a2(x : ctxt) : bool        {H.o : k2, H1.o : 3} 
 }.
 
 (* Or we can  give the restrictions at the top-level, e.g.: *)
-module type OAdvBis (H1 : Oracle, H : Oracle) 
+module type OAdvBis (H1 : Oracle, H : AOracle) 
   [a1 : {H.o, H1.o; H.o : k1, H1.o : 1 },
    a2 : {H.o, H1.o; H.o : k2, H1.o : 3 }]
  = {
-  proc a1(x : int) : int * int
-  
-  proc a2(x : int) : int
+  proc a1(p:pkey): (ptxt * ptxt)
+  proc a2(c:ctxt): bool
 }.
-(*****************)
+(*********************************************)
 
 (* Inverter *)
 module I (A : Adv) (H : Oracle) = {
-  var qs : int list
+  var qs : rand list
 
   module QRO = {
-    proc o (x : int) = {
-      var r : int;
+    proc o (x : rand) = {
+      var r;
       qs <- x :: qs;
       r <- H.o(x);
       return r;
@@ -72,13 +143,15 @@ module I (A : Adv) (H : Oracle) = {
   }
   module A0 = A(QRO)
 
-  proc invert(pk : int, y : int) : int = {
-    var m0,m1,b,x : int;
+  proc invert(pk : pkey, y : rand) : rand = {
+    var x, m0, m1, h, b;
 
     qs <- [];
-    (m0,m1) <- A0.a1(pk);    
-    b <- A0.a2(y);
-    x <- nth witness qs (find (fun _ => true) qs);
+    H.init();
+    (m0,m1) <- A0.a1(pk);  
+    h <$ dptxt;
+    b <- A0.a2(y || h);
+    x <- nth witness qs (find (fun p => f pk p = y) qs);
     return  x;
   }
 }.
@@ -91,10 +164,14 @@ section.
 
   local lemma bound_i :     
     choare[I0.invert: true ==> true] 
-    time [3 + 2 * k1 + 2 * k2; I(A,H).A0.a1 : 1; I(A,H).A0.a2 : 1; H.o : k1 + k2].
+    time [3 + 2 * k1 + 2 * k2; 
+          I0.A0.a1 : 1; 
+          I0.A0.a2 : 1; 
+          H.o : k1 + k2;
+          H.init : 1].
   proof.
   proc.
-  seq 3 : (size I.qs <= k1 + k2) [k1 + k2].
+  seq 5 : (size I.qs <= k1 + k2) [k1 + k2].
   call (_: true ;
     (I(A, H).QRO.o : size I.qs - k1)
     time
@@ -105,7 +182,11 @@ section.
   call (_: true; time).
   wp; skip => *. 
   split => /=; [1: by smt].
+  print cost_cons.
+  instantiate := (cost_cons {r : ptxt, x : rand} x : I.qs).
   admit.
+  print dptxt.
+  rnd.
   call (_: true;
     (I(A, H).QRO.o : size I.qs)
     time
@@ -116,13 +197,23 @@ section.
   split; [1: by smt].
   split; [2: by smt].
   admit.
-  wp; skip => *.
+  call (_: true; time); wp; skip => *.
   split => * /=; [1: by smt].
   split;
-  rewrite !big_constz !count_predT !size_range [smt (k1p k2p)].
+  rewrite !big_constz !count_predT !size_range. 
+  admit. (* [smt (k1p k2p)]. *)
+  by smt (k1p k2p).
   (* wp (size I.qs <= k1 + k2). *)  
   admit.
 qed.
+
+(* lemma foo: *)
+(* forall l, *)
+(* cost(_:{pk, y, m0, m1, b, x : bool})[I.qs = l :  *)
+(*     nth witness I.qs        *)
+(*     (find (fun (_ : int) => true) I.qs)] <= size l. *)
+(* proof. *)
+(* apply list_ind => /= => *. *)
 
 module A = { 
   proc g (x, y) : int = {
@@ -140,20 +231,20 @@ module A = {
   }
 }.
 
-lemma silly : choare[A.g : true ==> true] time [3].
+lemma foo : choare[A.g : true ==> true] time [3].
 proof.
 proc.
 wp; skip => *; split => //.
 admit.
 qed.
 
-lemma silly3 : choare[A.f : true ==> true] time [4].
+lemma foo3 : choare[A.f : true ==> true] time [4].
 proof.
 proc.
-call silly.
+call foo.
 (* Alternatively, we can do: *)
 (* call (_: true ==> true time [1]). *)
-(* apply silly. *)
+(* apply foo. *)
 wp; skip => *; split =>//.
 admit.
 qed.
@@ -173,7 +264,7 @@ module B = {
 }.
 
 (* For if statements, we add the cost of both branches. *)
-lemma silly4 : choare[B.f : true ==> true] time [5].
+lemma foo4 : choare[B.f : true ==> true] time [5].
 proof.
 proc.
 wp; skip => *; split => //.
@@ -191,7 +282,7 @@ module C = {
   }
 }.
 
-lemma silly5 : forall (a : int) (b : int), 
+lemma foo5 : forall (a : int) (b : int), 
 0 <= a /\ 0 <= b =>
 choare[C.f : x = a /\ y = b /\ x < y ==> true] time [2 * (a - b) + 1].
 proof.
@@ -212,8 +303,8 @@ admit.
   the maximal number of steps.  *)
 by smt.
 
-(* we prove that the invariant implies the post, and that the cost of all
- iterations is smaller than the final cost. *)
+(* We prove that the invariant implies the post, and that the cost of all
+  iterations is smaller than the final cost. *)
 skip => * => //; split; [1: by smt].
 rewrite !big_constz !count_predT !size_range. 
 print list_ind.
